ntor/Games.ec
@@ -268,7 +268,7 @@ module Game0 : GAKE_nodhs_i = {
           (* client instances can be ephkey revealed when pending if there isn't 
              a tested origin partner (agreeing on first message *)
         | Pending_mod st pk_e ir => {
-            if (untested_origins_c (pk_e, None) s_smap <> Some false) {
+            if (tested_origins_c (pk_e, None) s_smap <> Some true) {
               ek <- Some (st.`2);
               c_smap.[i] <- set_ir_eph (Pending_mod st pk_e ir);
             }
